Slight tightening up of printing

00Utils/Utils.thy
@@ -124,4 +124,11 @@ lemma [simp]: "x < y \<Longrightarrow> 1 < k \<Longrightarrow> Suc (k * x) < k *
   by (metis One_nat_def Suc_lessE Suc_lessI Suc_mult_less_cancel1 Suc_times_mod_eq 
             mod_mult_self1_is_0 nat.simps(3))
 
+fun opt_pair :: "('a \<rightharpoonup> 'b) \<Rightarrow> ('a \<rightharpoonup> 'c) \<Rightarrow> 'a \<rightharpoonup> 'b \<times> 'c" where
+  "opt_pair f g a = (case f a of
+      None \<Rightarrow> None
+    | Some b \<Rightarrow> (case g a of
+        None \<Rightarrow> None
+      | Some c \<Rightarrow> Some (b, c)))"
+
 end
