Correctness.thy
@@ -9,17 +9,17 @@ theorem tc_failure: "alg_compile e = None \<Longrightarrow>
   \<nexists>e\<^sub>t t. (Map.empty \<turnstile>\<^sub>n e\<^sub>t : t) \<and> tvarst e\<^sub>t = {} \<and> e = erase e\<^sub>t"
 proof -
   assume "alg_compile e = None"
-  hence "typecheck e = None" by simp
+  hence "typecheck e = None" by (simp split: option.splits)
   thus ?thesis by (metis typecheck_fails)
 qed
 
-theorem tc_terminationn: "alg_compile e = Some cd \<Longrightarrow> 
+theorem tc_terminationn: "alg_compile e = Some (cd, t) \<Longrightarrow> 
   \<exists>v. valn v \<and> e \<Down> v \<and> (\<exists>rs mem. rs R3 = 6 \<and> rs R4 = 3 \<and> 
     print_mval mem (mem 2) = print_nexpr v \<and> 
       iter (\<tturnstile> cd \<leadsto>\<^sub>m) (MS (case_reg 0 1 2 11 0) ((\<lambda>x. 0)(7 := 1)) (length cd)) (MS rs mem 0))"
 proof -
-  assume C: "alg_compile e = Some cd"
-  then obtain e\<^sub>t t where T: "typecheck e = Some (e\<^sub>t, t)" by fastforce
+  assume C: "alg_compile e = Some (cd, t)"
+  then obtain e\<^sub>t where T: "typecheck e = Some (e\<^sub>t, t)" by (auto split: option.splits prod.splits)
   hence TN: "(Map.empty \<turnstile>\<^sub>n e\<^sub>t : t) \<and> e = erase e\<^sub>t" by simp
   then obtain v\<^sub>t where ET: "e\<^sub>t \<Down>\<^sub>t v\<^sub>t" by fastforce
   hence VT: "valt v\<^sub>t" by simp
